refactor compilation to be recursive

experiments/meta/VerifiedTransform3.fst
@@ -92,8 +92,8 @@ type ast_exp =
 
 (** we only have one type, so probably this is not very useful **)
 type ast_typing : (e:ast_exp) -> (t:ast_typ) -> Type =
-  | C_IntTyping      : x:int -> ast_typing (EC_Int x) TInt
-  | AddTyping  : e1:ast_exp -> e2:ast_exp -> ast_typing e1 TInt -> ast_typing e2 TInt -> ast_typing (EAdd e1 e2) TInt
+  | C_IntTyping : x:int -> ast_typing (EC_Int x) TInt
+  | AddTyping   : e1:ast_exp -> e2:ast_exp -> ast_typing e1 TInt -> ast_typing e2 TInt -> ast_typing (EAdd e1 e2) TInt
 
 let t : ast_exp = EAdd (EC_Int 2) (EC_Int 1)
 
@@ -106,16 +106,6 @@ let _ = assert (sem t == 3)
 
 let c_int_typing (g:env) (x : int) : Tac (tot_typing g (pack (Tv_Const (C_Int x))) (`int)) =
   dyn_typing ()
-
-let fold_addition_lemma
-  (g:env)
-  (n m:int)
-  : Lemma (valid g (mk_eq2 (`int)
-                           (pack
-                             (Tv_App (Tv_App (`Prims.op_Addition) (pack (Tv_Const (C_Int n)), Q_Explicit))
-                                          (pack (Tv_Const (C_Int m)), Q_Explicit)))
-                           (pack (Tv_Const (C_Int (n+m))))))
-  = admit() // unsure if we can prove it statically, but could just call norm_term_env
 
 let mk_ec_int (g:env) (x:int) : e:term{
   tot_typing g e (`ast_exp) /\ 
@@ -131,38 +121,42 @@ let mk_ec_int (g:env) (x:int) : e:term{
   assume (valid g (mk_eq2 (`int) (pack (Tv_Const (C_Int x))) (`(sem (`#e)))));
   e
 
-let mk_eapp (g:env) (x:int) (y:int) : e:term{
+let mk_eapp (g:env) (x:term{tot_typing g x (`ast_exp)}) (y:term{tot_typing g y (`ast_exp)}) : e:term{
   tot_typing g e (`ast_exp) /\
   valid g (`(ast_typing (`#e) TInt)) /\
-  valid g (mk_eq2 (`int) (pack (Tv_Const (C_Int (x+y)))) (`(sem (`#e))))
+  valid g (mk_eq2 (`int) (`((sem (`#x)) + (sem (`#y)))) (`(sem (`#e))))
 } =
   let e = pack (
     Tv_App 
-      (Tv_App 
-        (`EAdd) 
-        (mk_ec_int g x, Q_Explicit))
-      (mk_ec_int g y, Q_Explicit)) in
+      (Tv_App (`EAdd) (x, Q_Explicit))
+      (y, Q_Explicit)) in
   assume (tot_typing g e (`ast_exp));
   assume (valid g (`(ast_typing (`#e) TInt)));
-  assume (valid g (mk_eq2 (`int) (pack (Tv_Const (C_Int (x+y)))) (`(sem (`#e)))));
+  assume (valid g (mk_eq2 (`int) (`((sem (`#x)) + (sem (`#y)))) (`(sem (`#e)))));
   e
 
+let compose_add (a b c d:int) : Lemma (requires (a == b /\ c == d)) (ensures (a+c == b+d)) = ()
 
-let rec cfold (g:env) (t0:term{tot_typing g t0 (`int)})
+let rec compile_to_ast (g:env) (t0:term{tot_typing g t0 (`int)})
   : TacP term (requires True)
               (ensures fun t1 -> 
-                tot_typing g t1 (`ast_exp) /\
-                valid g (`(ast_typing (`#t1) TInt)) /\
-                valid g (mk_eq2 (`int) t0 (`(sem (`#t1)))))
+                tot_typing g t1 (`ast_exp) /\                // AST syntax
+                valid g (`(ast_typing (`#t1) TInt)) /\       // well typed AST syntax
+                valid g (mk_eq2 (`int) t0 (`(sem (`#t1)))))  // equivalent semantics
 = 
   match inspect t0 with
   | Tv_FVar _ ->
     (* unfold *)
     let t1 = norm_term_env (`int) g [delta] t0 in
-    let t2 = cfold g t1 in
+    let t2 = compile_to_ast g t1 in
     eq2_trans g (`int) t0 t1 (`(sem (`#t2)));
     t2
-    
+  
+  | Tv_Const (C_Int x) ->
+    let t1 = mk_ec_int g x in
+    assume (valid g (mk_eq2 (`int) t0 (`(sem (`#t1)))));
+    t1
+
   (* detect ((op_Plus a) b) *)
   | Tv_App hd (a1, Q_Explicit) ->
     begin match inspect hd with
@@ -170,15 +164,26 @@ let rec cfold (g:env) (t0:term{tot_typing g t0 (`int)})
         begin match inspect op with
         | Tv_FVar fv ->
           if inspect_fv fv = ["Prims"; "op_Addition"]
-          then
-            match inspect a1, inspect a2 with
-            | Tv_Const (C_Int x), Tv_Const (C_Int y) ->
-              let t1 = mk_eapp g y x in
-              fold_addition_lemma g y x;
-              assume (valid g (mk_eq2 (`int) t0 (`(sem (`#t1))))); // use eq2_trans
-              t1
-            | _ ->  fail ("not implemented")
-          else fail ("not implemented")
+          then begin
+            assume (tot_typing g a1 (`int)); // need inversion lemma
+            assume (tot_typing g a2 (`int)); // need inversion lemma
+            let rhs = compile_to_ast g a1 in
+            let lhs = compile_to_ast g a2 in
+            let t1 = mk_eapp g lhs rhs in
+            // TODO:quotations and anti quotations are not stable
+            //  refactor this to use other techniques
+            //assert (valid g (mk_eq2 (`int) a1 (`(sem (`#rhs)))));
+            //assert (valid g (mk_eq2 (`int) a2 (`(sem (`#lhs)))));
+            assume (valid g (mk_eq2 (`int) (`((`#a1)+(`#a2))) (`(sem (`#lhs) + sem (`#rhs)))));
+            //assert (valid g (mk_eq2 (`int) (`(sem (`#lhs) + sem (`#rhs))) (`(sem (`#t1)))));
+            eq2_trans g (`int) (`((`#a1)+(`#a2))) (`(sem (`#lhs) + sem (`#rhs))) (`(sem (`#t1)));
+            assume (valid g (mk_eq2 (`int) t0 (`((`#a1)+(`#a2)))));
+            //assert (valid g (mk_eq2 (`int) (`((`#a1)+(`#a2))) (`(sem (`#t1)))));
+            admit (); //TODO: calling this lemma fails, which is weird. 
+            eq2_trans g (`int) t0 (`((`#a1)+(`#a2))) (`(sem (`#t1)));          
+            assert (valid g (mk_eq2 (`int) t0 (`(sem (`#t1)))));
+            t1
+          end else fail ("not implemented")
         | _ -> fail ("not implemented")
         end
       | _ -> fail ("not implemented")
@@ -189,7 +194,7 @@ let rec cfold (g:env) (t0:term{tot_typing g t0 (`int)})
 let specialize (nm':string) (e0:term) : dsl_tac_t = fun g ->
   let typ0 : tot_typing g e0 (`int) = dyn_typing () in
   FStar.Squash.return_squash typ0;
-  let e1 = cfold g e0 in
+  let e1 = compile_to_ast g e0 in
   let phi = mk_eq2 (`int) e0 (`(sem (`#e1))) in
   valid_wtf g phi;
   [
@@ -199,12 +204,18 @@ let specialize (nm':string) (e0:term) : dsl_tac_t = fun g ->
                     (mk_squash phi);
   ]
   
-let src1 : int = 4 + 5
+let src1 : int = 4 + 5 + 6
 
-%splice_t[tgt1; tgt1_pf] (specialize "tgt1" (`src1))
+%splice_t[tgt1;tgt1_pf] (specialize "tgt1" (`src1))
+
+// TODO: @Guido, here there is a universe problem. any tip on how to fix this?
+// let _ =
+//   FStar.Squash.give_proof tgt1_pf
 
 let _ = 
-  assert (tgt1 == EAdd (EC_Int 4) (EC_Int 5))
+  assert (tgt1 == EAdd (EAdd (EC_Int 4) (EC_Int 5)) (EC_Int 6));
+  assert (sem tgt1 == src1);
+  assert (sem tgt1 == 15) 
 
 [@expect_failure]
 let _ = 
